Capless/Weakening/TypedCont/Type.lean
@@ -1,9 +1,34 @@
 import Capless.Store
+import Capless.Weakening.Typing
 namespace Capless
+
+theorem EType.tweaken_ex (T : CType n m (k+1)) :
+  (EType.ex T).tweaken = EType.ex T.tweaken := by
+  simp [EType.tweaken, EType.trename, CType.tweaken]
+
+theorem EType.tweaken_type (T : CType n m k) :
+  (EType.type T).tweaken = EType.type T.tweaken := by
+  simp [EType.tweaken, EType.trename, CType.tweaken]
+
+theorem EType.tweaken_weaken (E : EType n m k) :
+  E.weaken.tweaken = E.tweaken.weaken := by
+  simp [EType.tweaken, EType.weaken, EType.trename_rename_comm]
 
 theorem TypedCont.tweaken
   (h : TypedCont Γ E t E') :
-  TypedCont (Γ.tvar S) E.tweaken t.tweaken E'.tweaken := sorry
-
+  TypedCont (Γ.tvar S) E.tweaken t.tweaken E'.tweaken := by
+  induction h
+  case none =>
+    simp [Cont.tweaken]
+    apply none
+  case cons ht _ ih =>
+    simp [Cont.tweaken]
+    simp [EType.tweaken_type]
+    apply cons
+    { have ht1 := ht.tweaken_ext (b := S)
+      rw [EType.tweaken_weaken] at ht1
+      exact ht1 }
+    { exact ih }
+  case conse => sorry
 
 end Capless
